<?xml version="1.0"?>
<rdf:RDF xmlns="http://www.semanticweb.org/delayed/cognitive-bias-ontology/BandwagonEffect#"
     xml:base="http://www.semanticweb.org/delayed/cognitive-bias-ontology/BandwagonEffect"
     xmlns:owl="http://www.w3.org/2002/07/owl#"
     xmlns:rdf="http://www.w3.org/1999/02/22-rdf-syntax-ns#"
     xmlns:xml="http://www.w3.org/XML/1998/namespace"
     xmlns:xsd="http://www.w3.org/2001/XMLSchema#"
     xmlns:rdfs="http://www.w3.org/2000/01/rdf-schema#"
     xmlns:terms="http://purl.org/dc/terms/"
     xmlns:affectedBy="https://w3id.org/affectedBy#"
     xmlns:BandwagonEffect="http://www.semanticweb.org/delayed/cognitive-bias-ontology/BandwagonEffect#">
    <owl:Ontology rdf:about="http://www.semanticweb.org/delayed/cognitive-bias-ontology/BandwagonEffect">
        <terms:creator xml:lang="en">Mirna Regolo</terms:creator>
        <terms:creator xml:lang="en">Stefano Renzetti</terms:creator>
        <terms:hasVersion xml:lang="en">0.1</terms:hasVersion>
        <rdfs:comment xml:lang="en">Bandwagon Effect Ontology</rdfs:comment>
        <rdfs:comment xml:lang="en">Bandwagon effect module of the Cognitive Bias Ontology.</rdfs:comment>
        <rdfs:comment xml:lang="en">The bandwagon effect is the tendency for people to adopt certain behaviors, styles, or attitudes simply because others are doing so. More specifically, it is a cognitive bias by which public opinion or behaviours can alter due to particular actions and beliefs rallying amongst the public.</rdfs:comment>
    </owl:Ontology>
    


    <!-- 
    ///////////////////////////////////////////////////////////////////////////////////////
    //
    // Annotation properties
    //
    ///////////////////////////////////////////////////////////////////////////////////////
     -->

    


    <!-- http://purl.org/dc/terms/creator -->

    <owl:AnnotationProperty rdf:about="http://purl.org/dc/terms/creator"/>
    


    <!-- http://purl.org/dc/terms/description -->

    <owl:AnnotationProperty rdf:about="http://purl.org/dc/terms/description"/>
    


    <!-- http://purl.org/dc/terms/hasVersion -->

    <owl:AnnotationProperty rdf:about="http://purl.org/dc/terms/hasVersion"/>
    


    <!-- http://purl.org/dc/terms/title -->

    <owl:AnnotationProperty rdf:about="http://purl.org/dc/terms/title"/>
    


    <!-- 
    ///////////////////////////////////////////////////////////////////////////////////////
    //
    // Object Properties
    //
    ///////////////////////////////////////////////////////////////////////////////////////
     -->

    


    <!-- http://www.ontologydesignpatterns.org/cp/owl/sequence.owl#precedes -->

    <owl:ObjectProperty rdf:about="http://www.ontologydesignpatterns.org/cp/owl/sequence.owl#precedes">
        <rdfs:domain rdf:resource="https://w3id.org/framester/data/framestercore/Popularity"/>
        <rdfs:range rdf:resource="https://w3id.org/framester/data/framestercore/SubjectiveInfluence"/>
        <rdfs:comment xml:lang="en">A relation between entities, expressing a &apos;sequence&apos; schema.</rdfs:comment>
    </owl:ObjectProperty>
    


    <!-- http://www.semanticweb.org/delayed/cognitive-bias-ontology/BandwagonEffect#isEngagedIn -->

    <owl:ObjectProperty rdf:about="http://www.semanticweb.org/delayed/cognitive-bias-ontology/BandwagonEffect#isEngagedIn">
        <rdfs:domain rdf:resource="http://www.ontologydesignpatterns.org/cp/owl/agentrole.owl#Agent"/>
        <rdfs:range rdf:resource="https://w3id.org/framester/data/framestercore/SubjectiveInfluence"/>
        <rdfs:comment xml:lang="en">To take part in some action, mental or physical.</rdfs:comment>
    </owl:ObjectProperty>
    


    <!-- https://w3id.org/affectedBy#influencedBy -->

    <owl:ObjectProperty rdf:about="https://w3id.org/affectedBy#influencedBy">
        <rdfs:domain rdf:resource="https://w3id.org/framester/data/framestercore/SubjectiveInfluence"/>
        <rdfs:range rdf:resource="https://w3id.org/framester/data/framestercore/Popularity"/>
        <rdfs:comment xml:lang="en">When something or someone is influenced by an external entity or factor.</rdfs:comment>
    </owl:ObjectProperty>
    


    <!-- 
    ///////////////////////////////////////////////////////////////////////////////////////
    //
    // Classes
    //
    ///////////////////////////////////////////////////////////////////////////////////////
     -->

    


    <!-- http://www.ontologydesignpatterns.org/cp/owl/agentrole.owl#Agent -->

    <owl:Class rdf:about="http://www.ontologydesignpatterns.org/cp/owl/agentrole.owl#Agent">
        <rdfs:comment xml:lang="en">Any physical or social agent, including a person, a social group, or an organization.</rdfs:comment>
    </owl:Class>
    


    <!-- https://w3id.org/framester/data/framestercore/Popularity -->

    <owl:Class rdf:about="https://w3id.org/framester/data/framestercore/Popularity">
        <rdfs:comment xml:lang="en">Degree of social approval or acceptance, influencing an agent&apos;s choices or actions.</rdfs:comment>
    </owl:Class>
    


    <!-- https://w3id.org/framester/data/framestercore/SubjectiveInfluence -->

    <owl:Class rdf:about="https://w3id.org/framester/data/framestercore/SubjectiveInfluence">
        <rdfs:comment xml:lang="en">An agent, situation or entity has an influence on another agent or entity.</rdfs:comment>
    </owl:Class>
    


    <!-- 
    ///////////////////////////////////////////////////////////////////////////////////////
    //
    // Individuals
    //
    ///////////////////////////////////////////////////////////////////////////////////////
     -->

    


    <!-- http://www.semanticweb.org/delayed/cognitive-bias-ontology/BandwagonEffect#bandwagon_effect -->

    <owl:NamedIndividual rdf:about="http://www.semanticweb.org/delayed/cognitive-bias-ontology/BandwagonEffect#bandwagon_effect">
        <rdf:type rdf:resource="https://w3id.org/framester/data/framestercore/SubjectiveInfluence"/>
        <affectedBy:influencedBy rdf:resource="http://www.semanticweb.org/delayed/cognitive-bias-ontology/BandwagonEffect#popular_thing"/>
    </owl:NamedIndividual>
    


    <!-- http://www.semanticweb.org/delayed/cognitive-bias-ontology/BandwagonEffect#decision-maker -->

    <owl:NamedIndividual rdf:about="http://www.semanticweb.org/delayed/cognitive-bias-ontology/BandwagonEffect#decision-maker">
        <rdf:type rdf:resource="http://www.ontologydesignpatterns.org/cp/owl/agentrole.owl#Agent"/>
        <isEngagedIn rdf:resource="http://www.semanticweb.org/delayed/cognitive-bias-ontology/BandwagonEffect#bandwagon_effect"/>
    </owl:NamedIndividual>
    


    <!-- http://www.semanticweb.org/delayed/cognitive-bias-ontology/BandwagonEffect#popular_thing -->

    <owl:NamedIndividual rdf:about="http://www.semanticweb.org/delayed/cognitive-bias-ontology/BandwagonEffect#popular_thing">
        <rdf:type rdf:resource="https://w3id.org/framester/data/framestercore/Popularity"/>
    </owl:NamedIndividual>
</rdf:RDF>



<!-- Generated by the OWL API (version 4.5.9.2019-02-01T07:24:44Z) https://github.com/owlcs/owlapi -->

