<?xml version="1.0"?>
<rdf:RDF xmlns="http://www.semanticweb.org/delayed/cognitive-bias-ontology/MoralCredentialEffect#"
     xml:base="http://www.semanticweb.org/delayed/cognitive-bias-ontology/MoralCredentialEffect"
     xmlns:owl="http://www.w3.org/2002/07/owl#"
     xmlns:rdf="http://www.w3.org/1999/02/22-rdf-syntax-ns#"
     xmlns:xml="http://www.w3.org/XML/1998/namespace"
     xmlns:xsd="http://www.w3.org/2001/XMLSchema#"
     xmlns:rdfs="http://www.w3.org/2000/01/rdf-schema#"
     xmlns:terms="http://purl.org/dc/terms/"
     xmlns:sequence="http://www.ontologydesignpatterns.org/cp/owl/sequence.owl#"
     xmlns:MoralCredentialEffect="http://www.semanticweb.org/delayed/cognitive-bias-ontology/MoralCredentialEffect#"
     xmlns:MoralCredentialEffect1="https://raw.githubusercontent.com/KRKE-Delayed/KRKE-cognitive-biases/main/cognitive-biases/ontology-modules/MoralCredentialEffect.owl#">
    <owl:Ontology rdf:about="https://raw.githubusercontent.com/KRKE-Delayed/KRKE-cognitive-biases/main/cognitive-biases/ontology-modules/MoralCredentialEffect.owl">
        <terms:creator xml:lang="en">Mirna Regolo</terms:creator>
        <terms:creator xml:lang="en">Stefano Renzetti</terms:creator>
        <terms:description xml:lang="en">Moral credential effect module of the Cognitive Bias Ontology.</terms:description>
        <terms:hasVersion xml:lang="en">0.1</terms:hasVersion>
        <terms:title xml:lang="en">Moral Credential Effect Ontology</terms:title>
        <rdfs:comment xml:lang="en">The Moral credential effect, is a bias that occurs when a person&apos;s track record as a good egalitarian establishes in them an unconscious ethical certification, endorsement, or license that increases the likelihood of less egalitarian decisions later. This effect occurs even when the audience or moral peer group is unaware of the affected person&apos;s previously established moral credential.</rdfs:comment>
    </owl:Ontology>
    


    <!-- 
    ///////////////////////////////////////////////////////////////////////////////////////
    //
    // Annotation properties
    //
    ///////////////////////////////////////////////////////////////////////////////////////
     -->

    


    <!-- http://purl.org/dc/terms/creator -->

    <owl:AnnotationProperty rdf:about="http://purl.org/dc/terms/creator"/>
    


    <!-- http://purl.org/dc/terms/description -->

    <owl:AnnotationProperty rdf:about="http://purl.org/dc/terms/description"/>
    


    <!-- http://purl.org/dc/terms/hasVersion -->

    <owl:AnnotationProperty rdf:about="http://purl.org/dc/terms/hasVersion"/>
    


    <!-- http://purl.org/dc/terms/title -->

    <owl:AnnotationProperty rdf:about="http://purl.org/dc/terms/title"/>
    


    <!-- 
    ///////////////////////////////////////////////////////////////////////////////////////
    //
    // Object Properties
    //
    ///////////////////////////////////////////////////////////////////////////////////////
     -->

    


    <!-- http://www.ontologydesignpatterns.org/cp/owl/classification.owl#isClassifiedBy -->

    <owl:ObjectProperty rdf:about="http://www.ontologydesignpatterns.org/cp/owl/classification.owl#isClassifiedBy">
        <rdfs:domain rdf:resource="https://w3id.org/framester/data/framestercore/Justifying"/>
        <rdfs:range rdf:resource="https://w3id.org/framester/data/framestercore/MoralityEvaluation"/>
        <rdfs:comment xml:lang="en">Used to describe information that is arranged by type.</rdfs:comment>
        <rdfs:label xml:lang="en">isClassifiedBy</rdfs:label>
    </owl:ObjectProperty>
    


    <!-- http://www.ontologydesignpatterns.org/cp/owl/sequence.owl#follows -->

    <owl:ObjectProperty rdf:about="http://www.ontologydesignpatterns.org/cp/owl/sequence.owl#follows">
        <rdfs:domain rdf:resource="https://w3id.org/framester/data/framestercore/Justifying"/>
        <rdfs:range rdf:resource="https://w3id.org/framester/data/framestercore/MoralityEvaluation"/>
        <rdfs:comment xml:lang="en">A relation between entities, expressing a &apos;sequence&apos; schema.</rdfs:comment>
        <rdfs:label xml:lang="en">follows</rdfs:label>
    </owl:ObjectProperty>
    


    <!-- http://www.ontologydesignpatterns.org/cp/owl/sequence.owl#precedes -->

    <owl:ObjectProperty rdf:about="http://www.ontologydesignpatterns.org/cp/owl/sequence.owl#precedes">
        <rdfs:domain rdf:resource="https://raw.githubusercontent.com/KRKE-Delayed/KRKE-cognitive-biases/main/cognitive-biases/ontology-modules/MoralCredentialEffect.owl#PreviousMoralAction"/>
        <rdfs:range rdf:resource="https://w3id.org/framester/data/framestercore/MoralityEvaluation"/>
        <rdfs:comment xml:lang="en">A relation between entities, expressing a &apos;sequence&apos; schema.</rdfs:comment>
        <rdfs:label xml:lang="en">precedes</rdfs:label>
    </owl:ObjectProperty>
    


    <!-- https://raw.githubusercontent.com/KRKE-Delayed/KRKE-cognitive-biases/main/cognitive-biases/ontology-modules/MoralCredentialEffect.owl#hasPreviousMoralAction -->

    <owl:ObjectProperty rdf:about="https://raw.githubusercontent.com/KRKE-Delayed/KRKE-cognitive-biases/main/cognitive-biases/ontology-modules/MoralCredentialEffect.owl#hasPreviousMoralAction">
        <rdfs:domain rdf:resource="https://w3id.org/framester/data/framestercore/Justifying"/>
        <rdfs:range rdf:resource="https://raw.githubusercontent.com/KRKE-Delayed/KRKE-cognitive-biases/main/cognitive-biases/ontology-modules/MoralCredentialEffect.owl#PreviousMoralAction"/>
        <rdfs:comment xml:lang="en">Indicates that someone has performed a moral action in the past, which may have an impact on their current decisions or behaviors.</rdfs:comment>
        <rdfs:label xml:lang="en">hasPreviousMoralAction</rdfs:label>
    </owl:ObjectProperty>
    


    <!-- https://raw.githubusercontent.com/KRKE-Delayed/KRKE-cognitive-biases/main/cognitive-biases/ontology-modules/MoralCredentialEffect.owl#isEngagedIn -->

    <owl:ObjectProperty rdf:about="https://raw.githubusercontent.com/KRKE-Delayed/KRKE-cognitive-biases/main/cognitive-biases/ontology-modules/MoralCredentialEffect.owl#isEngagedIn">
        <rdfs:domain rdf:resource="http://www.ontologydesignpatterns.org/cp/owl/agentrole.owl#Agent"/>
        <rdfs:range rdf:resource="https://w3id.org/framester/data/framestercore/Justifying"/>
        <rdfs:comment xml:lang="en">To take part in some action, mental or physical.</rdfs:comment>
        <rdfs:label xml:lang="en">isEngagedIn</rdfs:label>
    </owl:ObjectProperty>
    


    <!-- 
    ///////////////////////////////////////////////////////////////////////////////////////
    //
    // Classes
    //
    ///////////////////////////////////////////////////////////////////////////////////////
     -->

    


    <!-- http://www.ontologydesignpatterns.org/cp/owl/agentrole.owl#Agent -->

    <owl:Class rdf:about="http://www.ontologydesignpatterns.org/cp/owl/agentrole.owl#Agent">
        <rdfs:comment xml:lang="en">Any physical or social agent, including a person, a social group, or an organization.</rdfs:comment>
        <rdfs:label xml:lang="en">Agent</rdfs:label>
    </owl:Class>
    


    <!-- https://raw.githubusercontent.com/KRKE-Delayed/KRKE-cognitive-biases/main/cognitive-biases/ontology-modules/MoralCredentialEffect.owl#PreviousMoralAction -->

    <owl:Class rdf:about="https://raw.githubusercontent.com/KRKE-Delayed/KRKE-cognitive-biases/main/cognitive-biases/ontology-modules/MoralCredentialEffect.owl#PreviousMoralAction">
        <rdfs:comment xml:lang="en">Refers to a moral action performed by someone in the past, which may influence the agent&apos;s current decisions or behaviors.</rdfs:comment>
        <rdfs:label xml:lang="en">PreviousMoralAction</rdfs:label>
    </owl:Class>
    


    <!-- https://w3id.org/framester/data/framestercore/Justifying -->

    <owl:Class rdf:about="https://w3id.org/framester/data/framestercore/Justifying">
        <rdfs:comment xml:lang="en">To show that something is reasonable, right, or true.</rdfs:comment>
        <rdfs:label xml:lang="en">Justifying</rdfs:label>
    </owl:Class>
    


    <!-- https://w3id.org/framester/data/framestercore/MoralityEvaluation -->

    <owl:Class rdf:about="https://w3id.org/framester/data/framestercore/MoralityEvaluation">
        <rdfs:comment xml:lang="en">An evaluation with respect to the morality or rightness of his or her behavior.</rdfs:comment>
        <rdfs:label xml:lang="en">MoralityEvaluation</rdfs:label>
    </owl:Class>
    


    <!-- 
    ///////////////////////////////////////////////////////////////////////////////////////
    //
    // Individuals
    //
    ///////////////////////////////////////////////////////////////////////////////////////
     -->

    


    <!-- https://raw.githubusercontent.com/KRKE-Delayed/KRKE-cognitive-biases/main/cognitive-biases/ontology-modules/MoralCredentialEffect.owl#decision-maker -->

    <owl:NamedIndividual rdf:about="https://raw.githubusercontent.com/KRKE-Delayed/KRKE-cognitive-biases/main/cognitive-biases/ontology-modules/MoralCredentialEffect.owl#decision-maker">
        <rdf:type rdf:resource="http://www.ontologydesignpatterns.org/cp/owl/agentrole.owl#Agent"/>
        <MoralCredentialEffect1:isEngagedIn rdf:resource="https://raw.githubusercontent.com/KRKE-Delayed/KRKE-cognitive-biases/main/cognitive-biases/ontology-modules/MoralCredentialEffect.owl#justifying"/>
        <rdfs:label xml:lang="en">decision-maker</rdfs:label>
    </owl:NamedIndividual>
    


    <!-- https://raw.githubusercontent.com/KRKE-Delayed/KRKE-cognitive-biases/main/cognitive-biases/ontology-modules/MoralCredentialEffect.owl#justifying -->

    <owl:NamedIndividual rdf:about="https://raw.githubusercontent.com/KRKE-Delayed/KRKE-cognitive-biases/main/cognitive-biases/ontology-modules/MoralCredentialEffect.owl#justifying">
        <rdf:type rdf:resource="https://w3id.org/framester/data/framestercore/Justifying"/>
        <MoralCredentialEffect1:hasPreviousMoralAction rdf:resource="https://raw.githubusercontent.com/KRKE-Delayed/KRKE-cognitive-biases/main/cognitive-biases/ontology-modules/MoralCredentialEffect.owl#previous_moral_action"/>
        <rdfs:label xml:lang="en">justifying</rdfs:label>
    </owl:NamedIndividual>
    


    <!-- https://raw.githubusercontent.com/KRKE-Delayed/KRKE-cognitive-biases/main/cognitive-biases/ontology-modules/MoralCredentialEffect.owl#morality_evaluation -->

    <owl:NamedIndividual rdf:about="https://raw.githubusercontent.com/KRKE-Delayed/KRKE-cognitive-biases/main/cognitive-biases/ontology-modules/MoralCredentialEffect.owl#morality_evaluation">
        <rdf:type rdf:resource="https://w3id.org/framester/data/framestercore/MoralityEvaluation"/>
        <sequence:follows rdf:resource="https://raw.githubusercontent.com/KRKE-Delayed/KRKE-cognitive-biases/main/cognitive-biases/ontology-modules/MoralCredentialEffect.owl#previous_moral_action"/>
        <rdfs:label xml:lang="en">morality_evaluation</rdfs:label>
    </owl:NamedIndividual>
    


    <!-- https://raw.githubusercontent.com/KRKE-Delayed/KRKE-cognitive-biases/main/cognitive-biases/ontology-modules/MoralCredentialEffect.owl#previous_moral_action -->

    <owl:NamedIndividual rdf:about="https://raw.githubusercontent.com/KRKE-Delayed/KRKE-cognitive-biases/main/cognitive-biases/ontology-modules/MoralCredentialEffect.owl#previous_moral_action">
        <rdf:type rdf:resource="https://raw.githubusercontent.com/KRKE-Delayed/KRKE-cognitive-biases/main/cognitive-biases/ontology-modules/MoralCredentialEffect.owl#PreviousMoralAction"/>
        <rdfs:label xml:lang="en">previous_moral_action</rdfs:label>
    </owl:NamedIndividual>
</rdf:RDF>



<!-- Generated by the OWL API (version 4.5.9.2019-02-01T07:24:44Z) https://github.com/owlcs/owlapi -->

