<?xml version="1.0"?>
<rdf:RDF xmlns="http://www.semanticweb.org/delayed/cognitive-bias-ontology/PlaceboEffect#"
     xml:base="http://www.semanticweb.org/delayed/cognitive-bias-ontology/PlaceboEffect"
     xmlns:owl="http://www.w3.org/2002/07/owl#"
     xmlns:rdf="http://www.w3.org/1999/02/22-rdf-syntax-ns#"
     xmlns:xml="http://www.w3.org/XML/1998/namespace"
     xmlns:xsd="http://www.w3.org/2001/XMLSchema#"
     xmlns:rdfs="http://www.w3.org/2000/01/rdf-schema#"
     xmlns:terms="http://purl.org/dc/terms/"
     xmlns:PlaceboEffect="http://www.semanticweb.org/delayed/cognitive-bias-ontology/PlaceboEffect#">
    <owl:Ontology rdf:about="http://www.semanticweb.org/delayed/cognitive-bias-ontology/PlaceboEffect">
        <terms:creator xml:lang="en">Mirna Regolo</terms:creator>
        <terms:creator xml:lang="en">Stefano Renzetti</terms:creator>
        <terms:description xml:lang="en">Placebo effect module of the Cognitive Bias Ontology.</terms:description>
        <terms:hasVersion xml:lang="en">0.1</terms:hasVersion>
        <terms:title xml:lang="en">Placebo Effect Ontology</terms:title>
        <rdfs:comment xml:lang="en">The &quot;Placebo effect&quot; bias refers to a cognitive bias in which an individual experiences a perceived improvement in their condition or symptoms after receiving a treatment or intervention that has no therapeutic effect.</rdfs:comment>
    </owl:Ontology>
    


    <!-- 
    ///////////////////////////////////////////////////////////////////////////////////////
    //
    // Annotation properties
    //
    ///////////////////////////////////////////////////////////////////////////////////////
     -->

    


    <!-- http://purl.org/dc/terms/creator -->

    <owl:AnnotationProperty rdf:about="http://purl.org/dc/terms/creator"/>
    


    <!-- http://purl.org/dc/terms/description -->

    <owl:AnnotationProperty rdf:about="http://purl.org/dc/terms/description"/>
    


    <!-- http://purl.org/dc/terms/hasVersion -->

    <owl:AnnotationProperty rdf:about="http://purl.org/dc/terms/hasVersion"/>
    


    <!-- http://purl.org/dc/terms/title -->

    <owl:AnnotationProperty rdf:about="http://purl.org/dc/terms/title"/>
    


    <!-- 
    ///////////////////////////////////////////////////////////////////////////////////////
    //
    // Object Properties
    //
    ///////////////////////////////////////////////////////////////////////////////////////
     -->

    


    <!-- http://www.ontologydesignpatterns.org/cp/owl/sequence.owl#follows -->

    <owl:ObjectProperty rdf:about="http://www.ontologydesignpatterns.org/cp/owl/sequence.owl#follows">
        <rdfs:domain rdf:resource="https://w3id.org/framester/data/framestercore/UndergoChange"/>
        <rdfs:range rdf:resource="https://w3id.org/framester/data/framestercore/MentalProperty"/>
        <rdfs:comment xml:lang="en">A relation between entities, expressing a &apos;sequence&apos; schema.</rdfs:comment>
    </owl:ObjectProperty>
    


    <!-- http://www.semanticweb.org/delayed/cognitive-bias-ontology/PlaceboEffect#causesChange -->

    <owl:ObjectProperty rdf:about="http://www.semanticweb.org/delayed/cognitive-bias-ontology/PlaceboEffect#causesChange">
        <rdfs:domain rdf:resource="http://www.ontologydesignpatterns.org/cp/owl/agentrole.owl#Agent"/>
        <rdfs:range rdf:resource="http://www.ontologydesignpatterns.org/cp/owl/agentrole.owl#Agent"/>
        <rdfs:comment xml:lang="en">A property that indicates the cause of an entity&apos;s alteration or modification, leading to changes in its category membership or attribute values.</rdfs:comment>
    </owl:ObjectProperty>
    


    <!-- http://www.semanticweb.org/delayed/cognitive-bias-ontology/PlaceboEffect#usesMentalProperty -->

    <owl:ObjectProperty rdf:about="http://www.semanticweb.org/delayed/cognitive-bias-ontology/PlaceboEffect#usesMentalProperty">
        <rdfs:domain rdf:resource="http://www.ontologydesignpatterns.org/cp/owl/agentrole.owl#Agent"/>
        <rdfs:range rdf:resource="https://w3id.org/framester/data/framestercore/MentalProperty"/>
        <rdfs:comment xml:lang="en">A property that signifies an agent&apos;s engagement with a mental attribute, concept, or state as part of a cognitive process or decision-making.</rdfs:comment>
    </owl:ObjectProperty>
    


    <!-- https://w3id.org/affectedBy#influencedBy -->

    <owl:ObjectProperty rdf:about="https://w3id.org/affectedBy#influencedBy">
        <rdfs:domain rdf:resource="https://w3id.org/framester/data/framestercore/UndergoChange"/>
        <rdfs:range rdf:resource="http://www.ontologydesignpatterns.org/cp/owl/agentrole.owl#Agent"/>
        <rdfs:comment xml:lang="en">When something or someone is influenced by an external entity or factor.</rdfs:comment>
    </owl:ObjectProperty>
    


    <!-- 
    ///////////////////////////////////////////////////////////////////////////////////////
    //
    // Classes
    //
    ///////////////////////////////////////////////////////////////////////////////////////
     -->

    


    <!-- http://www.ontologydesignpatterns.org/cp/owl/agentrole.owl#Agent -->

    <owl:Class rdf:about="http://www.ontologydesignpatterns.org/cp/owl/agentrole.owl#Agent">
        <rdfs:comment xml:lang="en">Any physical or social agent, including a person, a social group, or an organization.</rdfs:comment>
    </owl:Class>
    


    <!-- https://w3id.org/framester/data/framestercore/MentalProperty -->

    <owl:Class rdf:about="https://w3id.org/framester/data/framestercore/MentalProperty">
        <rdfs:comment xml:lang="en">Mental attribute or state associated with an entity.</rdfs:comment>
    </owl:Class>
    


    <!-- https://w3id.org/framester/data/framestercore/UndergoChange -->

    <owl:Class rdf:about="https://w3id.org/framester/data/framestercore/UndergoChange">
        <rdfs:comment xml:lang="en">An entity changes, either in its category membership or in terms of the value of an attribute.</rdfs:comment>
    </owl:Class>
    


    <!-- 
    ///////////////////////////////////////////////////////////////////////////////////////
    //
    // Individuals
    //
    ///////////////////////////////////////////////////////////////////////////////////////
     -->

    


    <!-- http://www.semanticweb.org/delayed/cognitive-bias-ontology/PlaceboEffect#decision-maker -->

    <owl:NamedIndividual rdf:about="http://www.semanticweb.org/delayed/cognitive-bias-ontology/PlaceboEffect#decision-maker">
        <rdf:type rdf:resource="http://www.ontologydesignpatterns.org/cp/owl/agentrole.owl#Agent"/>
        <causesChange rdf:resource="http://www.semanticweb.org/delayed/cognitive-bias-ontology/PlaceboEffect#decision-maker"/>
        <usesMentalProperty rdf:resource="http://www.semanticweb.org/delayed/cognitive-bias-ontology/PlaceboEffect#mental_property"/>
    </owl:NamedIndividual>
    


    <!-- http://www.semanticweb.org/delayed/cognitive-bias-ontology/PlaceboEffect#mental_property -->

    <owl:NamedIndividual rdf:about="http://www.semanticweb.org/delayed/cognitive-bias-ontology/PlaceboEffect#mental_property">
        <rdf:type rdf:resource="https://w3id.org/framester/data/framestercore/MentalProperty"/>
    </owl:NamedIndividual>
</rdf:RDF>



<!-- Generated by the OWL API (version 4.5.9.2019-02-01T07:24:44Z) https://github.com/owlcs/owlapi -->

