<?xml version="1.0"?>
<rdf:RDF xmlns="http://www.semanticweb.org/delayed/cognitive-bias-ontology/ReversePsychology#"
     xml:base="http://www.semanticweb.org/delayed/cognitive-bias-ontology/ReversePsychology"
     xmlns:owl="http://www.w3.org/2002/07/owl#"
     xmlns:rdf="http://www.w3.org/1999/02/22-rdf-syntax-ns#"
     xmlns:xml="http://www.w3.org/XML/1998/namespace"
     xmlns:xsd="http://www.w3.org/2001/XMLSchema#"
     xmlns:rdfs="http://www.w3.org/2000/01/rdf-schema#"
     xmlns:terms="http://purl.org/dc/terms/"
     xmlns:ReversePsychology="http://www.semanticweb.org/delayed/cognitive-bias-ontology/ReversePsychology#">
    <owl:Ontology rdf:about="http://www.semanticweb.org/delayed/cognitive-bias-ontology/ReversePsychology">
        <terms:creator xml:lang="en">Mirna Regolo</terms:creator>
        <terms:creator xml:lang="en">Stefano Renzetti</terms:creator>
        <terms:description xml:lang="en">Reverse psycology module of the Cognitive Bias Ontology</terms:description>
        <terms:hasVersion xml:lang="en">0.1</terms:hasVersion>
        <terms:title xml:lang="en">Reverse Psychology Ontology</terms:title>
        <rdfs:comment xml:lang="en">Reverse psychology is a technique involving the assertion of a belief or behavior that is opposite to the one desired, with the expectation that this approach will encourage the subject of the persuasion to do what is actually desired.</rdfs:comment>
    </owl:Ontology>
    


    <!-- 
    ///////////////////////////////////////////////////////////////////////////////////////
    //
    // Annotation properties
    //
    ///////////////////////////////////////////////////////////////////////////////////////
     -->

    


    <!-- http://purl.org/dc/terms/creator -->

    <owl:AnnotationProperty rdf:about="http://purl.org/dc/terms/creator"/>
    


    <!-- http://purl.org/dc/terms/description -->

    <owl:AnnotationProperty rdf:about="http://purl.org/dc/terms/description"/>
    


    <!-- http://purl.org/dc/terms/hasVersion -->

    <owl:AnnotationProperty rdf:about="http://purl.org/dc/terms/hasVersion"/>
    


    <!-- http://purl.org/dc/terms/title -->

    <owl:AnnotationProperty rdf:about="http://purl.org/dc/terms/title"/>
    


    <!-- http://www.w3.org/2000/01/rdf-schema#comment -->

    <owl:AnnotationProperty rdf:about="http://www.w3.org/2000/01/rdf-schema#comment"/>
    


    <!-- 
    ///////////////////////////////////////////////////////////////////////////////////////
    //
    // Object Properties
    //
    ///////////////////////////////////////////////////////////////////////////////////////
     -->

    


    <!-- http://www.ontologydesignpatterns.org/cp/owl/partof.owl#hasPart -->

    <owl:ObjectProperty rdf:about="http://www.ontologydesignpatterns.org/cp/owl/partof.owl#hasPart">
        <rdfs:domain rdf:resource="https://w3id.org/framester/data/framestercore/Cogitation"/>
        <rdfs:range rdf:resource="https://w3id.org/framester/data/framestercore/SubjectiveInfluence"/>
        <rdfs:comment xml:lang="en">A transitive relation expressing parthood between any entities.</rdfs:comment>
    </owl:ObjectProperty>
    


    <!-- http://www.ontologydesignpatterns.org/cp/owl/partof.owl#isPartOf -->

    <owl:ObjectProperty rdf:about="http://www.ontologydesignpatterns.org/cp/owl/partof.owl#isPartOf">
        <rdfs:domain rdf:resource="https://w3id.org/framester/data/framestercore/SubjectiveInfluence"/>
        <rdfs:range rdf:resource="https://w3id.org/framester/data/framestercore/Cogitation"/>
        <rdfs:comment xml:lang="en">A transitive relation expressing parthood between any entities.</rdfs:comment>
    </owl:ObjectProperty>
    


    <!-- http://www.ontologydesignpatterns.org/cp/owl/sequence.owl#follows -->

    <owl:ObjectProperty rdf:about="http://www.ontologydesignpatterns.org/cp/owl/sequence.owl#follows">
        <rdfs:domain rdf:resource="https://w3id.org/framester/data/framestercore/Response"/>
        <rdfs:range rdf:resource="https://w3id.org/framester/data/framestercore/Cogitation"/>
        <rdfs:comment xml:lang="en">A relation between entities, expressing a &apos;sequence&apos; schema.</rdfs:comment>
    </owl:ObjectProperty>
    


    <!-- http://www.semanticweb.org/delayed/cognitive-bias-ontology/ReversePsychology#hasResponse -->

    <owl:ObjectProperty rdf:about="http://www.semanticweb.org/delayed/cognitive-bias-ontology/ReversePsychology#hasResponse">
        <rdfs:domain rdf:resource="https://w3id.org/framester/data/framestercore/SubjectiveInfluence"/>
        <rdfs:range rdf:resource="https://w3id.org/framester/data/framestercore/Response"/>
    </owl:ObjectProperty>
    


    <!-- http://www.semanticweb.org/delayed/cognitive-bias-ontology/ReversePsychology#influencesResponseOf -->

    <owl:ObjectProperty rdf:about="http://www.semanticweb.org/delayed/cognitive-bias-ontology/ReversePsychology#influencesResponseOf">
        <rdfs:domain rdf:resource="https://w3id.org/framester/data/framestercore/SubjectiveInfluence"/>
        <rdfs:range rdf:resource="http://www.ontologydesignpatterns.org/cp/owl/agentrole.owl#Agent"/>
        <rdfs:comment xml:lang="en">Indicates what external or internal factor influences a response, is the cause of a reation.</rdfs:comment>
    </owl:ObjectProperty>
    


    <!-- https://w3id.org/affectedBy#influencedBy -->

    <owl:ObjectProperty rdf:about="https://w3id.org/affectedBy#influencedBy">
        <rdfs:domain rdf:resource="https://w3id.org/framester/data/framestercore/Response"/>
        <rdfs:range rdf:resource="https://w3id.org/framester/data/framestercore/SubjectiveInfluence"/>
        <rdfs:comment xml:lang="en">When an agent&apos;s decision is influenced by an external entity.</rdfs:comment>
    </owl:ObjectProperty>
    


    <!-- 
    ///////////////////////////////////////////////////////////////////////////////////////
    //
    // Classes
    //
    ///////////////////////////////////////////////////////////////////////////////////////
     -->

    


    <!-- http://www.ontologydesignpatterns.org/cp/owl/agentrole.owl#Agent -->

    <owl:Class rdf:about="http://www.ontologydesignpatterns.org/cp/owl/agentrole.owl#Agent">
        <rdfs:comment xml:lang="en">Any physical or social agent, including a person, a social group, or an organization.</rdfs:comment>
    </owl:Class>
    


    <!-- https://w3id.org/framester/data/framestercore/Cogitation -->

    <owl:Class rdf:about="https://w3id.org/framester/data/framestercore/Cogitation">
        <rdfs:comment xml:lang="en">The act of thinking about a subject.</rdfs:comment>
    </owl:Class>
    


    <!-- https://w3id.org/framester/data/framestercore/Response -->

    <owl:Class rdf:about="https://w3id.org/framester/data/framestercore/Response">
        <rdfs:comment xml:lang="en">An answer or reaction.</rdfs:comment>
    </owl:Class>
    


    <!-- https://w3id.org/framester/data/framestercore/SubjectiveInfluence -->

    <owl:Class rdf:about="https://w3id.org/framester/data/framestercore/SubjectiveInfluence">
        <rdfs:comment xml:lang="en">Based on or influenced by personal feelings, tastes, or opinions.</rdfs:comment>
    </owl:Class>
    


    <!-- 
    ///////////////////////////////////////////////////////////////////////////////////////
    //
    // Individuals
    //
    ///////////////////////////////////////////////////////////////////////////////////////
     -->

    


    <!-- http://www.semanticweb.org/delayed/cognitive-bias-ontology/ReversePsychology#decision-maker -->

    <owl:NamedIndividual rdf:about="http://www.semanticweb.org/delayed/cognitive-bias-ontology/ReversePsychology#decision-maker">
        <rdf:type rdf:resource="http://www.ontologydesignpatterns.org/cp/owl/agentrole.owl#Agent"/>
        <rdfs:comment xml:lang="en">Represents individuals or entities (Agent) who make decisions influenced by biases, including the status quo bias.</rdfs:comment>
    </owl:NamedIndividual>
    


    <!-- http://www.semanticweb.org/delayed/cognitive-bias-ontology/ReversePsychology#response -->

    <owl:NamedIndividual rdf:about="http://www.semanticweb.org/delayed/cognitive-bias-ontology/ReversePsychology#response">
        <rdf:type rdf:resource="https://w3id.org/framester/data/framestercore/Response"/>
        <rdfs:comment xml:lang="en">An answer or reaction influenced by the reverse psychology.</rdfs:comment>
    </owl:NamedIndividual>
    


    <!-- http://www.semanticweb.org/delayed/cognitive-bias-ontology/ReversePsychology#reverse_psychology -->

    <owl:NamedIndividual rdf:about="http://www.semanticweb.org/delayed/cognitive-bias-ontology/ReversePsychology#reverse_psychology">
        <rdf:type rdf:resource="https://w3id.org/framester/data/framestercore/SubjectiveInfluence"/>
        <hasResponse rdf:resource="http://www.semanticweb.org/delayed/cognitive-bias-ontology/ReversePsychology#response"/>
        <influencesResponseOf rdf:resource="http://www.semanticweb.org/delayed/cognitive-bias-ontology/ReversePsychology#decision-maker"/>
        <rdfs:comment xml:lang="en">The psychological technique that influences the response.</rdfs:comment>
    </owl:NamedIndividual>
</rdf:RDF>



<!-- Generated by the OWL API (version 4.5.9.2019-02-01T07:24:44Z) https://github.com/owlcs/owlapi -->

