<?xml version="1.0"?>
<rdf:RDF xmlns="http://www.semanticweb.org/delayed/cognitive-bias-ontology/StatusQuoBias#"
     xml:base="http://www.semanticweb.org/delayed/cognitive-bias-ontology/StatusQuoBias"
     xmlns:owl="http://www.w3.org/2002/07/owl#"
     xmlns:rdf="http://www.w3.org/1999/02/22-rdf-syntax-ns#"
     xmlns:xml="http://www.w3.org/XML/1998/namespace"
     xmlns:xsd="http://www.w3.org/2001/XMLSchema#"
     xmlns:rdfs="http://www.w3.org/2000/01/rdf-schema#"
     xmlns:terms="http://purl.org/dc/terms/"
     xmlns:sequence="http://www.ontologydesignpatterns.org/cp/owl/sequence.owl#"
     xmlns:affectedBy="https://w3id.org/affectedBy#"
     xmlns:StatusQuoBias="http://www.semanticweb.org/delayed/cognitive-bias-ontology/StatusQuoBias#">
    <owl:Ontology rdf:about="http://www.semanticweb.org/delayed/cognitive-bias-ontology/StatusQuoBias">
        <terms:creator xml:lang="en">Mirna Regolo</terms:creator>
        <terms:creator xml:lang="en">Stefano Renzetti</terms:creator>
        <terms:description xml:lang="en">Status quo bias module of the Cognitive Bias Ontology</terms:description>
        <terms:hasVersion xml:lang="en">0.1</terms:hasVersion>
        <terms:title xml:lang="en">Status Quo Bias Ontology</terms:title>
        <rdfs:comment xml:lang="en">Status quo bias is an emotional bias; a preference for the maintenance of one&apos;s current or previous state of affairs, or a preference to not undertake any action to change this current or previous state.</rdfs:comment>
    </owl:Ontology>
    


    <!-- 
    ///////////////////////////////////////////////////////////////////////////////////////
    //
    // Annotation properties
    //
    ///////////////////////////////////////////////////////////////////////////////////////
     -->

    


    <!-- http://purl.org/dc/terms/creator -->

    <owl:AnnotationProperty rdf:about="http://purl.org/dc/terms/creator"/>
    


    <!-- http://purl.org/dc/terms/description -->

    <owl:AnnotationProperty rdf:about="http://purl.org/dc/terms/description"/>
    


    <!-- http://purl.org/dc/terms/hasVersion -->

    <owl:AnnotationProperty rdf:about="http://purl.org/dc/terms/hasVersion"/>
    


    <!-- http://purl.org/dc/terms/title -->

    <owl:AnnotationProperty rdf:about="http://purl.org/dc/terms/title"/>
    


    <!-- 
    ///////////////////////////////////////////////////////////////////////////////////////
    //
    // Object Properties
    //
    ///////////////////////////////////////////////////////////////////////////////////////
     -->

    


    <!-- http://www.ontologydesignpatterns.org/cp/owl/partof.owl#isPartOf -->

    <owl:ObjectProperty rdf:about="http://www.ontologydesignpatterns.org/cp/owl/partof.owl#isPartOf">
        <rdfs:domain rdf:resource="https://w3id.org/framester/data/framestercore/Choosing"/>
        <rdfs:range rdf:resource="https://w3id.org/framester/data/framestercore/Cogitation"/>
        <rdfs:comment xml:lang="en">A transitive relation expressing parthood between any entities.</rdfs:comment>
    </owl:ObjectProperty>
    


    <!-- http://www.ontologydesignpatterns.org/cp/owl/sequence.owl#follows -->

    <owl:ObjectProperty rdf:about="http://www.ontologydesignpatterns.org/cp/owl/sequence.owl#follows">
        <rdfs:domain rdf:resource="https://w3id.org/framester/data/framestercore/Choosing"/>
        <rdfs:range rdf:resource="https://w3id.org/framester/data/framestercore/Cogitation"/>
        <rdfs:comment xml:lang="en">A relation between entities, expressing a &apos;sequence&apos; schema.</rdfs:comment>
    </owl:ObjectProperty>
    


    <!-- http://www.ontologydesignpatterns.org/cp/owl/sequence.owl#precedes -->

    <owl:ObjectProperty rdf:about="http://www.ontologydesignpatterns.org/cp/owl/sequence.owl#precedes">
        <rdfs:domain rdf:resource="http://www.semanticweb.org/delayed/cognitive-bias-ontology/StatusQuoBias#Alternative"/>
        <rdfs:domain rdf:resource="https://w3id.org/framester/data/framestercore/Choosing"/>
        <rdfs:range rdf:resource="https://w3id.org/framester/data/framestercore/Choosing"/>
        <rdfs:range rdf:resource="https://w3id.org/framester/data/framestercore/Preserving"/>
        <rdfs:comment xml:lang="en">A relation between entities, expressing a &apos;sequence&apos; schema.</rdfs:comment>
    </owl:ObjectProperty>
    


    <!-- http://www.semanticweb.org/delayed/cognitive-bias-ontology/StatusQuoBias#choosingAlternative -->

    <owl:ObjectProperty rdf:about="http://www.semanticweb.org/delayed/cognitive-bias-ontology/StatusQuoBias#choosingAlternative">
        <rdfs:domain rdf:resource="http://www.ontologydesignpatterns.org/cp/owl/agentrole.owl#Agent"/>
        <rdfs:range rdf:resource="https://w3id.org/framester/data/framestercore/Choosing"/>
        <rdfs:comment xml:lang="en">The act to decide what you want from two or more things or possibilities.</rdfs:comment>
    </owl:ObjectProperty>
    


    <!-- https://w3id.org/affectedBy#affectedBy -->

    <owl:ObjectProperty rdf:about="https://w3id.org/affectedBy#affectedBy">
        <rdfs:domain rdf:resource="https://w3id.org/framester/data/framestercore/Choosing"/>
        <rdfs:range rdf:resource="https://w3id.org/framester/data/framestercore/Custom"/>
        <rdfs:comment xml:lang="en">A relation between qualities or entities.</rdfs:comment>
    </owl:ObjectProperty>
    


    <!-- 
    ///////////////////////////////////////////////////////////////////////////////////////
    //
    // Classes
    //
    ///////////////////////////////////////////////////////////////////////////////////////
     -->

    


    <!-- http://www.ontologydesignpatterns.org/cp/owl/agentrole.owl#Agent -->

    <owl:Class rdf:about="http://www.ontologydesignpatterns.org/cp/owl/agentrole.owl#Agent">
        <rdfs:comment xml:lang="en">Any physical or social agent, including a person, a social group, or an organization.</rdfs:comment>
    </owl:Class>
    


    <!-- http://www.semanticweb.org/delayed/cognitive-bias-ontology/StatusQuoBias#Alternative -->

    <owl:Class rdf:about="http://www.semanticweb.org/delayed/cognitive-bias-ontology/StatusQuoBias#Alternative">
        <rdfs:comment xml:lang="en">A physical or mental object that represents a choice between two or more things.</rdfs:comment>
    </owl:Class>
    


    <!-- http://www.semanticweb.org/delayed/cognitive-bias-ontology/StatusQuoBias#NewAlternative -->

    <owl:Class rdf:about="http://www.semanticweb.org/delayed/cognitive-bias-ontology/StatusQuoBias#NewAlternative">
        <rdfs:subClassOf rdf:resource="http://www.semanticweb.org/delayed/cognitive-bias-ontology/StatusQuoBias#Alternative"/>
    </owl:Class>
    


    <!-- http://www.semanticweb.org/delayed/cognitive-bias-ontology/StatusQuoBias#StatusQuoAlternative -->

    <owl:Class rdf:about="http://www.semanticweb.org/delayed/cognitive-bias-ontology/StatusQuoBias#StatusQuoAlternative">
        <rdfs:subClassOf rdf:resource="http://www.semanticweb.org/delayed/cognitive-bias-ontology/StatusQuoBias#Alternative"/>
    </owl:Class>
    


    <!-- https://w3id.org/framester/data/framestercore/Choosing -->

    <owl:Class rdf:about="https://w3id.org/framester/data/framestercore/Choosing">
        <rdfs:comment xml:lang="en">To decide what you want from two or more things or possibilities.</rdfs:comment>
    </owl:Class>
    


    <!-- https://w3id.org/framester/data/framestercore/Cogitation -->

    <owl:Class rdf:about="https://w3id.org/framester/data/framestercore/Cogitation">
        <rdfs:comment xml:lang="en">The act of thinking about a subject.</rdfs:comment>
    </owl:Class>
    


    <!-- https://w3id.org/framester/data/framestercore/Custom -->

    <owl:Class rdf:about="https://w3id.org/framester/data/framestercore/Custom">
        <rdfs:comment xml:lang="en">A way of behaving or a belief that has been established for a long time.</rdfs:comment>
    </owl:Class>
    


    <!-- https://w3id.org/framester/data/framestercore/Preserving -->

    <owl:Class rdf:about="https://w3id.org/framester/data/framestercore/Preserving">
        <rdfs:comment xml:lang="en">To keep something as it is, especially in order to prevent it from decaying or being damaged or destroyed.</rdfs:comment>
    </owl:Class>
    


    <!-- 
    ///////////////////////////////////////////////////////////////////////////////////////
    //
    // Individuals
    //
    ///////////////////////////////////////////////////////////////////////////////////////
     -->

    


    <!-- http://www.semanticweb.org/delayed/cognitive-bias-ontology/StatusQuoBias#decision_maker -->

    <owl:NamedIndividual rdf:about="http://www.semanticweb.org/delayed/cognitive-bias-ontology/StatusQuoBias#decision_maker">
        <rdf:type rdf:resource="http://www.ontologydesignpatterns.org/cp/owl/agentrole.owl#Agent"/>
        <choosingAlternative rdf:resource="http://www.semanticweb.org/delayed/cognitive-bias-ontology/StatusQuoBias#status_quo_alternative"/>
        <affectedBy:affectedBy rdf:resource="http://www.semanticweb.org/delayed/cognitive-bias-ontology/StatusQuoBias#stereotype"/>
        <rdfs:comment xml:lang="en">Represents individuals or entities (Agent) who make decisions influenced by biases, including the status quo bias.</rdfs:comment>
    </owl:NamedIndividual>
    


    <!-- http://www.semanticweb.org/delayed/cognitive-bias-ontology/StatusQuoBias#new_alternative -->

    <owl:NamedIndividual rdf:about="http://www.semanticweb.org/delayed/cognitive-bias-ontology/StatusQuoBias#new_alternative">
        <rdf:type rdf:resource="http://www.semanticweb.org/delayed/cognitive-bias-ontology/StatusQuoBias#NewAlternative"/>
        <sequence:follows rdf:resource="http://www.semanticweb.org/delayed/cognitive-bias-ontology/StatusQuoBias#status_quo_alternative"/>
        <rdfs:comment xml:lang="en">The alternative challenging the StatusQuoAlternative.</rdfs:comment>
    </owl:NamedIndividual>
    


    <!-- http://www.semanticweb.org/delayed/cognitive-bias-ontology/StatusQuoBias#status_quo_alternative -->

    <owl:NamedIndividual rdf:about="http://www.semanticweb.org/delayed/cognitive-bias-ontology/StatusQuoBias#status_quo_alternative">
        <rdf:type rdf:resource="http://www.semanticweb.org/delayed/cognitive-bias-ontology/StatusQuoBias#StatusQuoAlternative"/>
        <sequence:precedes rdf:resource="http://www.semanticweb.org/delayed/cognitive-bias-ontology/StatusQuoBias#new_alternative"/>
        <rdfs:comment xml:lang="en">The alternative influenced by stereotype.</rdfs:comment>
    </owl:NamedIndividual>
    


    <!-- http://www.semanticweb.org/delayed/cognitive-bias-ontology/StatusQuoBias#stereotype -->

    <owl:NamedIndividual rdf:about="http://www.semanticweb.org/delayed/cognitive-bias-ontology/StatusQuoBias#stereotype">
        <rdf:type rdf:resource="https://w3id.org/framester/data/framestercore/Custom"/>
        <affectedBy:affectedBy rdf:resource="http://www.semanticweb.org/delayed/cognitive-bias-ontology/StatusQuoBias#status_quo_alternative"/>
        <rdfs:comment xml:lang="en">The alternative relative to traditional norms or customs.</rdfs:comment>
    </owl:NamedIndividual>
</rdf:RDF>



<!-- Generated by the OWL API (version 4.5.9.2019-02-01T07:24:44Z) https://github.com/owlcs/owlapi -->

