<?xml version="1.0"?>
<rdf:RDF xmlns="http://www.semanticweb.org/delayed/cognitive-bias-ontology/UltimateAttributionError#"
     xml:base="http://www.semanticweb.org/delayed/cognitive-bias-ontology/UltimateAttributionError"
     xmlns:owl="http://www.w3.org/2002/07/owl#"
     xmlns:rdf="http://www.w3.org/1999/02/22-rdf-syntax-ns#"
     xmlns:xml="http://www.w3.org/XML/1998/namespace"
     xmlns:xsd="http://www.w3.org/2001/XMLSchema#"
     xmlns:rdfs="http://www.w3.org/2000/01/rdf-schema#"
     xmlns:terms="http://purl.org/dc/terms/"
     xmlns:affectedBy="https://w3id.org/affectedBy#"
     xmlns:UltimateAttributionError="http://www.semanticweb.org/delayed/cognitive-bias-ontology/UltimateAttributionError#"
     xmlns:UltimateAttributionError1="https://raw.githubusercontent.com/KRKE-Delayed/KRKE-cognitive-biases/main/cognitive-biases/ontology-modules/UltimateAttributionError.owl#">
    <owl:Ontology rdf:about="https://raw.githubusercontent.com/KRKE-Delayed/KRKE-cognitive-biases/main/cognitive-biases/ontology-modules/UltimateAttributionError.owl">
        <terms:creator xml:lang="en">Mirna Regolo</terms:creator>
        <terms:creator xml:lang="en">Stefano Renzetti</terms:creator>
        <terms:description xml:lang="en">Ultimate attribution error module of the Cognitive Bias Ontology.</terms:description>
        <terms:hasVersion xml:lang="en">0.1</terms:hasVersion>
        <terms:title xml:lang="en">Ultimate Attribution Error Ontology</terms:title>
        <rdfs:comment xml:lang="en">The Ultimate Attribution Error, also known as Ultimate Attribution Fallacy, is a psychological concept that refers to a cognitive bias in which individuals tend to attribute the behavior of members of other groups (out-groups) to their inherent traits or characteristics, while attributing the behavior of members of their own group (in-group) to external factors or situational influences.</rdfs:comment>
    </owl:Ontology>
    


    <!-- 
    ///////////////////////////////////////////////////////////////////////////////////////
    //
    // Annotation properties
    //
    ///////////////////////////////////////////////////////////////////////////////////////
     -->

    


    <!-- http://purl.org/dc/terms/creator -->

    <owl:AnnotationProperty rdf:about="http://purl.org/dc/terms/creator"/>
    


    <!-- http://purl.org/dc/terms/description -->

    <owl:AnnotationProperty rdf:about="http://purl.org/dc/terms/description"/>
    


    <!-- http://purl.org/dc/terms/hasVersion -->

    <owl:AnnotationProperty rdf:about="http://purl.org/dc/terms/hasVersion"/>
    


    <!-- http://purl.org/dc/terms/title -->

    <owl:AnnotationProperty rdf:about="http://purl.org/dc/terms/title"/>
    


    <!-- 
    ///////////////////////////////////////////////////////////////////////////////////////
    //
    // Object Properties
    //
    ///////////////////////////////////////////////////////////////////////////////////////
     -->

    


    <!-- http://www.ontologydesignpatterns.org/cp/owl/sequence.owl#follows -->

    <owl:ObjectProperty rdf:about="http://www.ontologydesignpatterns.org/cp/owl/sequence.owl#follows">
        <rdfs:domain rdf:resource="https://w3id.org/framester/data/framestercore/Differentiation"/>
        <rdfs:range rdf:resource="https://w3id.org/framester/data/framestercore/SuccessOrFailure"/>
        <rdfs:comment xml:lang="en">A relation between entities, expressing a &apos;sequence&apos; schema.</rdfs:comment>
        <rdfs:label xml:lang="en">follows</rdfs:label>
    </owl:ObjectProperty>
    


    <!-- https://raw.githubusercontent.com/KRKE-Delayed/KRKE-cognitive-biases/main/cognitive-biases/ontology-modules/UltimateAttributionError.owl#isEngagedIn -->

    <owl:ObjectProperty rdf:about="https://raw.githubusercontent.com/KRKE-Delayed/KRKE-cognitive-biases/main/cognitive-biases/ontology-modules/UltimateAttributionError.owl#isEngagedIn">
        <rdfs:domain rdf:resource="http://www.ontologydesignpatterns.org/cp/owl/agentrole.owl#Agent"/>
        <rdfs:range rdf:resource="https://w3id.org/framester/data/framestercore/PerceptionExperience"/>
        <rdfs:comment xml:lang="en">To take part in some action, mental or physical.</rdfs:comment>
        <rdfs:label xml:lang="en">isEngagedIn</rdfs:label>
    </owl:ObjectProperty>
    


    <!-- https://w3id.org/affectedBy#influencedBy -->

    <owl:ObjectProperty rdf:about="https://w3id.org/affectedBy#influencedBy">
        <rdfs:domain rdf:resource="https://w3id.org/framester/data/framestercore/PerceptionExperience"/>
        <rdfs:range rdf:resource="https://w3id.org/framester/data/framestercore/SuccessOrFailure"/>
        <rdfs:comment xml:lang="en">When something or someone is influenced by an external entity or factor.</rdfs:comment>
        <rdfs:label xml:lang="en">influencedBy</rdfs:label>
    </owl:ObjectProperty>
    


    <!-- 
    ///////////////////////////////////////////////////////////////////////////////////////
    //
    // Classes
    //
    ///////////////////////////////////////////////////////////////////////////////////////
     -->

    


    <!-- http://www.ontologydesignpatterns.org/cp/owl/agentrole.owl#Agent -->

    <owl:Class rdf:about="http://www.ontologydesignpatterns.org/cp/owl/agentrole.owl#Agent">
        <rdfs:comment xml:lang="en">Any physical or social agent, including a person, a social group, or an organization.</rdfs:comment>
        <rdfs:label xml:lang="en">Agent</rdfs:label>
    </owl:Class>
    


    <!-- https://w3id.org/framester/data/framestercore/Differentiation -->

    <owl:Class rdf:about="https://w3id.org/framester/data/framestercore/Differentiation">
        <rdfs:comment xml:lang="en">Being aware (or not being aware) of the difference between more phenomena, which may be expressed jointly or disjointly.</rdfs:comment>
        <rdfs:label xml:lang="en">Differentiation</rdfs:label>
    </owl:Class>
    


    <!-- https://w3id.org/framester/data/framestercore/PerceptionExperience -->

    <owl:Class rdf:about="https://w3id.org/framester/data/framestercore/PerceptionExperience">
        <owl:equivalentClass>
            <owl:Class>
                <owl:intersectionOf rdf:parseType="Collection">
                    <rdf:Description rdf:about="https://w3id.org/framester/data/framestercore/Differentiation"/>
                    <rdf:Description rdf:about="https://w3id.org/framester/data/framestercore/PerceptionExperience"/>
                    <rdf:Description rdf:about="https://w3id.org/framester/data/framestercore/SuccessOrFailure"/>
                </owl:intersectionOf>
            </owl:Class>
        </owl:equivalentClass>
        <rdfs:label xml:lang="en">PerceptionExperience</rdfs:label>
    </owl:Class>
    


    <!-- https://w3id.org/framester/data/framestercore/SuccessOrFailure -->

    <owl:Class rdf:about="https://w3id.org/framester/data/framestercore/SuccessOrFailure">
        <rdfs:comment xml:lang="en">The outcome or result of a particular endeavor, which can be either positive (success) or negative (failure).</rdfs:comment>
        <rdfs:label xml:lang="en">SuccessOrFailure</rdfs:label>
    </owl:Class>
    


    <!-- 
    ///////////////////////////////////////////////////////////////////////////////////////
    //
    // Individuals
    //
    ///////////////////////////////////////////////////////////////////////////////////////
     -->

    


    <!-- https://raw.githubusercontent.com/KRKE-Delayed/KRKE-cognitive-biases/main/cognitive-biases/ontology-modules/UltimateAttributionError.owl#decision-maker -->

    <owl:NamedIndividual rdf:about="https://raw.githubusercontent.com/KRKE-Delayed/KRKE-cognitive-biases/main/cognitive-biases/ontology-modules/UltimateAttributionError.owl#decision-maker">
        <rdf:type rdf:resource="http://www.ontologydesignpatterns.org/cp/owl/agentrole.owl#Agent"/>
        <UltimateAttributionError1:isEngagedIn rdf:resource="https://raw.githubusercontent.com/KRKE-Delayed/KRKE-cognitive-biases/main/cognitive-biases/ontology-modules/UltimateAttributionError.owl#ultimate_attribution_error"/>
        <rdfs:label xml:lang="en">decision-maker</rdfs:label>
    </owl:NamedIndividual>
    


    <!-- https://raw.githubusercontent.com/KRKE-Delayed/KRKE-cognitive-biases/main/cognitive-biases/ontology-modules/UltimateAttributionError.owl#success_or_fail -->

    <owl:NamedIndividual rdf:about="https://raw.githubusercontent.com/KRKE-Delayed/KRKE-cognitive-biases/main/cognitive-biases/ontology-modules/UltimateAttributionError.owl#success_or_fail">
        <rdf:type rdf:resource="https://w3id.org/framester/data/framestercore/SuccessOrFailure"/>
        <rdfs:label xml:lang="en">success_or_fail</rdfs:label>
    </owl:NamedIndividual>
    


    <!-- https://raw.githubusercontent.com/KRKE-Delayed/KRKE-cognitive-biases/main/cognitive-biases/ontology-modules/UltimateAttributionError.owl#ultimate_attribution_error -->

    <owl:NamedIndividual rdf:about="https://raw.githubusercontent.com/KRKE-Delayed/KRKE-cognitive-biases/main/cognitive-biases/ontology-modules/UltimateAttributionError.owl#ultimate_attribution_error">
        <rdf:type rdf:resource="https://w3id.org/framester/data/framestercore/PerceptionExperience"/>
        <affectedBy:influencedBy rdf:resource="https://raw.githubusercontent.com/KRKE-Delayed/KRKE-cognitive-biases/main/cognitive-biases/ontology-modules/UltimateAttributionError.owl#success_or_fail"/>
        <rdfs:label xml:lang="en">ultimate_attribution_error</rdfs:label>
    </owl:NamedIndividual>
</rdf:RDF>



<!-- Generated by the OWL API (version 4.5.9.2019-02-01T07:24:44Z) https://github.com/owlcs/owlapi -->

